theories/UniPolicies/LLFOptimality.v
@@ -9,13 +9,13 @@ Require Import SchedulerInterface.
 Require Import SchedulingAlgorithmInterface.
 Require Import SchedulingAlgorithmSchedulerBridge.
 Require Import SchedulingAlgorithmCanonicalBridge.
+Require Import SchedulingAlgorithmNormalization.
+Require Import SchedulingAlgorithmOptimalitySkeleton.
 Require Import UniPolicies.MetricChooserLemmas.
 Require Import UniPolicies.LLF.
 Require Import UniPolicies.LLFLemmas.
 Require Import UniPolicies.LLFTransform.
 Import ListNotations.
-
-(* ===== Section 8: Strong normalization ===== *)
 
 Lemma repair_pushes_first_violation_forward_llf :
   forall J (candidates_of : CandidateSource)
@@ -61,6 +61,44 @@ Proof.
   - subst t. exact Hmatch.
 Qed.
 
+Lemma llf_canonical_at_dec :
+  forall candidates_of jobs sched t,
+    {matches_choose_llf_at_with jobs candidates_of sched t} +
+    {~ matches_choose_llf_at_with jobs candidates_of sched t}.
+Proof.
+  intros candidates_of jobs sched t.
+  destruct (is_llf_canonical_at_b candidates_of jobs sched t) eqn:Hb.
+  - left. apply (is_llf_canonical_at_b_true_iff candidates_of jobs sched t). exact Hb.
+  - right. apply (is_llf_canonical_at_b_false_iff candidates_of jobs sched t). exact Hb.
+Qed.
+
+Definition LLFCanonicalRepairSpec
+    (J : JobId -> Prop)
+    (candidates_of : CandidateSource)
+    (cand_spec : CandidateSourceSpec J candidates_of)
+    (jobs : JobId -> Job) :
+    CanonicalRepairSpec llf_generic_spec J candidates_of jobs.
+Proof.
+  refine ({|
+    canonical_at := fun sched t => matches_choose_llf_at_with jobs candidates_of sched t;
+    canonical_before := fun sched H => matches_choose_llf_before jobs candidates_of sched H;
+    canonical_before_def := _;
+    canonical_at_def := _;
+    canonical_at_dec := _;
+    repair_non_canonical := _;
+    repair_pushes_forward := _
+  |}).
+  - intros sched H. tauto.
+  - intros sched t. tauto.
+  - intros sched t. apply llf_canonical_at_dec.
+  - intros J_bool sched t HJbool Hvalid Hfeas HJonly Hcpu Hnot.
+    exact (repair_non_canonical_at_llf J J_bool candidates_of cand_spec jobs sched t
+             HJbool Hvalid Hfeas HJonly Hcpu Hnot).
+  - intros sched sched' t Hcpu Hcpu' Hagree Hcanon Hat.
+    exact (repair_pushes_first_violation_forward_llf J candidates_of cand_spec
+             jobs sched sched' t Hcpu Hcpu' Hagree Hcanon Hat).
+Defined.
+
 Lemma llf_normalize_to_canonical :
   forall J (J_bool : JobId -> bool) (candidates_of : CandidateSource)
          (cand_spec : CandidateSourceSpec J candidates_of)
@@ -77,174 +115,19 @@ Lemma llf_normalize_to_canonical :
       single_cpu_only sched' /\
       matches_choose_llf_before jobs candidates_of sched' H.
 Proof.
-  intros J J_bool candidates_of cand_spec jobs sched H HJbool.
-  induction H as [| H' IH].
-  - intros Hvalid Hfeas HJonly Hcpu1.
-    exists sched.
-    refine (conj Hvalid (conj Hfeas (conj HJonly (conj Hcpu1 _)))).
-    unfold matches_choose_llf_before, matches_dispatch_before.
-    intros t Hlt. lia.
-  - intros Hvalid Hfeas HJonly Hcpu1.
-    destruct (IH Hvalid Hfeas HJonly Hcpu1)
-      as [sched_ih [Hih_valid [Hih_feas [Hih_Jonly [Hih_cpu1 Hih_canon]]]]].
-    destruct (is_llf_canonical_at_b candidates_of jobs sched_ih H') eqn:Hb.
-    + exists sched_ih.
-      refine (conj Hih_valid (conj Hih_feas (conj Hih_Jonly (conj Hih_cpu1 _)))).
-      unfold matches_choose_llf_before, matches_dispatch_before.
-      intros t Hlt.
-      assert (Hcases : t < H' \/ t = H') by lia.
-      destruct Hcases as [Hlt' | Heq].
-      * exact (Hih_canon t Hlt').
-      * subst t.
-        apply (is_llf_canonical_at_b_true_iff candidates_of jobs sched_ih H').
-        exact Hb.
-    + assert (Hnot : ~ matches_choose_llf_at_with jobs candidates_of sched_ih H').
-      { apply (is_llf_canonical_at_b_false_iff candidates_of jobs sched_ih H'). exact Hb. }
-      destruct (repair_non_canonical_at_llf J J_bool candidates_of cand_spec
-                   jobs sched_ih H'
-                   HJbool Hih_valid Hih_feas Hih_Jonly Hih_cpu1 Hnot)
-        as [sched_r [Hr_valid [Hr_feas [Hr_Jonly [Hr_cpu1 [Hr_agree Hr_match]]]]]].
-      exists sched_r.
-      refine (conj Hr_valid (conj Hr_feas (conj Hr_Jonly (conj Hr_cpu1 _)))).
-      exact (repair_pushes_first_violation_forward_llf
-               J candidates_of cand_spec
-               jobs sched_ih sched_r H'
-               Hih_cpu1 Hr_cpu1 Hr_agree Hr_match Hih_canon).
+  intros J J_bool candidates_of cand_spec jobs sched H HJbool Hvalid Hfeas HJonly Hcpu.
+  eapply normalize_to_canonical_generic with
+      (alg := llf_generic_spec)
+      (cand_spec := cand_spec)
+      (J_bool := J_bool)
+      (sched := sched).
+  - exact (LLFCanonicalRepairSpec J candidates_of cand_spec jobs).
+  - exact HJbool.
+  - exact Hvalid.
+  - exact Hfeas.
+  - exact HJonly.
+  - exact Hcpu.
 Qed.
-
-Lemma llf_normalize_up_to :
-  forall J (J_bool : JobId -> bool) (candidates_of : CandidateSource)
-         (cand_spec : CandidateSourceSpec J candidates_of)
-         jobs sched H,
-    (forall x, J_bool x = true <-> J x) ->
-    valid_schedule jobs 1 sched ->
-    feasible_schedule_on J jobs 1 sched ->
-    (forall t j, sched t 0 = Some j -> J j) ->
-    single_cpu_only sched ->
-    exists sched',
-      valid_schedule jobs 1 sched' /\
-      feasible_schedule_on J jobs 1 sched' /\
-      (forall t, t < H -> matches_choose_llf_at_with jobs candidates_of sched' t).
-Proof.
-  intros J J_bool candidates_of cand_spec jobs sched H
-         HJbool Hvalid Hfeas HJonly Hcpu1.
-  destruct (llf_normalize_to_canonical
-              J J_bool candidates_of cand_spec jobs sched H
-              HJbool Hvalid Hfeas HJonly Hcpu1)
-    as [sched' [Hvalid' [Hfeas' [_HJonly' [_Hcpu1' Hcanon]]]]].
-  exists sched'.
-  split. exact Hvalid'.
-  split. exact Hfeas'.
-  exact Hcanon.
-Qed.
-
-(* ===== Section 9: Truncation ===== *)
-
-Definition trunc_sched (sched : Schedule) (H : nat) : Schedule :=
-  fun t c => if t <? H then sched t c else None.
-
-Lemma trunc_sched_before : forall sched H t c,
-    t < H -> trunc_sched sched H t c = sched t c.
-Proof.
-  intros sched H t c Hlt.
-  unfold trunc_sched.
-  assert (E : (t <? H) = true) by (apply Nat.ltb_lt; exact Hlt).
-  rewrite E. reflexivity.
-Qed.
-
-Lemma trunc_sched_after : forall sched H t c,
-    H <= t -> trunc_sched sched H t c = None.
-Proof.
-  intros sched H t c Hle.
-  unfold trunc_sched.
-  destruct (t <? H) eqn:E.
-  - apply Nat.ltb_lt in E. lia.
-  - reflexivity.
-Qed.
-
-Lemma trunc_sched_single_cpu_only : forall sched H,
-    single_cpu_only sched ->
-    single_cpu_only (trunc_sched sched H).
-Proof.
-  intros sched H Honly t c Hc.
-  unfold trunc_sched.
-  destruct (t <? H) eqn:E.
-  - exact (Honly t c Hc).
-  - reflexivity.
-Qed.
-
-Lemma trunc_sched_valid : forall jobs sched H,
-    valid_schedule jobs 1 sched ->
-    valid_schedule jobs 1 (trunc_sched sched H).
-Proof.
-  intros jobs sched H Hvalid j t c Hc Hrun.
-  assert (Hc0 : c = 0) by lia. subst c.
-  destruct (lt_dec t H) as [Hlt | Hge].
-  - rewrite (trunc_sched_before sched H t 0 Hlt) in Hrun.
-    assert (Helig : eligible jobs 1 sched j t) by exact (Hvalid j t 0 Hc Hrun).
-    split.
-    + exact (proj1 Helig).
-    + intro Hcomp. apply (proj2 Helig). unfold completed in *.
-      assert (Heq : service_job 1 (trunc_sched sched H) j t =
-                    service_job 1 sched j t).
-      { apply service_job_eq_of_cpu_count_eq. intros t'' Hlt''.
-        destruct (lt_dec t'' H) as [Hlt''' | Hge'''].
-        - simpl. unfold runs_on. rewrite (trunc_sched_before sched H t'' 0 Hlt'''). reflexivity.
-        - exfalso. lia. }
-      rewrite Heq in Hcomp. exact Hcomp.
-  - rewrite (trunc_sched_after sched H t 0 (proj1 (Nat.nlt_ge t H) Hge)) in Hrun.
-    discriminate.
-Qed.
-
-Lemma trunc_sched_feasible : forall J jobs sched H,
-    (forall j, J j -> job_abs_deadline (jobs j) <= H) ->
-    feasible_schedule_on J jobs 1 sched ->
-    feasible_schedule_on J jobs 1 (trunc_sched sched H).
-Proof.
-  intros J jobs sched H Hdl_le Hfeas j HJj Hmiss.
-  apply (Hfeas j HJj).
-  unfold missed_deadline in *. unfold completed in *.
-  assert (Heq : service_job 1 (trunc_sched sched H) j (job_abs_deadline (jobs j)) =
-                service_job 1 sched j (job_abs_deadline (jobs j))).
-  { apply service_job_eq_of_cpu_count_eq. intros t Hlt.
-    destruct (lt_dec t H) as [Hlt' | Hge'].
-    - simpl. unfold runs_on. rewrite (trunc_sched_before sched H t 0 Hlt'). reflexivity.
-    - assert (Hge : H <= t) by lia.
-      assert (Hdl : job_abs_deadline (jobs j) <= H) by (exact (Hdl_le j HJj)).
-      assert (HH : job_abs_deadline (jobs j) <= t) by lia.
-      lia. }
-  rewrite <- Heq. exact Hmiss.
-Qed.
-
-Lemma trunc_sched_llf_canonical :
-  forall J (candidates_of : CandidateSource)
-         (cand_spec : CandidateSourceSpec J candidates_of)
-         jobs sched H,
-    single_cpu_only sched ->
-    single_cpu_only (trunc_sched sched H) ->
-    matches_choose_llf_before jobs candidates_of sched H ->
-    matches_choose_llf_before jobs candidates_of (trunc_sched sched H) H.
-Proof.
-  intros J candidates_of cand_spec jobs sched H Honly Htrunc_only Hcanon.
-  unfold matches_choose_llf_before, matches_dispatch_before,
-         matches_choose_llf_at_with, matches_dispatch_at_with.
-  simpl.
-  intros t Hlt.
-  rewrite (trunc_sched_before sched H t 0 Hlt).
-  assert (Hagree : agrees_before (trunc_sched sched H) sched t).
-  { intros t' c Hlt''.
-    rewrite (trunc_sched_before sched H t' c (Nat.lt_trans t' t H Hlt'' Hlt)).
-    reflexivity. }
-  assert (Hagree_sym : agrees_before sched (trunc_sched sched H) t)
-    by (exact (agrees_before_sym _ _ _ Hagree)).
-  rewrite (candidates_of_agrees_before J candidates_of cand_spec jobs
-             (trunc_sched sched H) sched t Hagree).
-  rewrite (choose_llf_agrees_before jobs (trunc_sched sched H) sched t _
-             Hagree).
-  exact (Hcanon t Hlt).
-Qed.
-
-(* ===== Section 10: Bridge to scheduler_rel ===== *)
 
 Lemma canonical_and_idle_implies_scheduler_rel_llf :
   forall J enumJ (candidates_of : CandidateSource)
@@ -264,8 +147,6 @@ Proof.
   eapply canonical_and_idle_implies_scheduler_rel_generic; eauto.
 Qed.
 
-(* ===== Section 11: Main theorem ===== *)
-
 Theorem llf_optimality_on_finite_jobs :
   forall J (J_bool : JobId -> bool) enumJ
          (candidates_of : CandidateSource)
@@ -278,47 +159,18 @@ Theorem llf_optimality_on_finite_jobs :
     schedulable_by_on J (llf_scheduler candidates_of) jobs 1.
 Proof.
   intros J J_bool enumJ candidates_of cand_spec jobs
-         HJbool HJ_in HJ_complete Hfeas_on.
-  destruct Hfeas_on as [sched0 [Hvalid0 Hfeas0]].
-  set (sched1 := J_restrict J_bool (mk_single_cpu sched0)).
-  assert (Hvalid1 : valid_schedule jobs 1 sched1).
-  { unfold sched1.
-    apply (J_restrict_valid J_bool J jobs (mk_single_cpu sched0) HJbool).
-    exact (mk_single_cpu_valid jobs sched0 Hvalid0). }
-  assert (Hfeas1 : feasible_schedule_on J jobs 1 sched1).
-  { unfold sched1.
-    apply (J_restrict_feasible J_bool J jobs (mk_single_cpu sched0) HJbool).
-    exact (mk_single_cpu_feasible J jobs sched0 Hfeas0). }
-  assert (HJonly1 : forall t j, sched1 t 0 = Some j -> J j).
-  { intros t j Hrun. unfold sched1 in Hrun.
-    exact (J_restrict_J_only J_bool J (mk_single_cpu sched0) t j HJbool Hrun). }
-  assert (Hcpu1 : single_cpu_only sched1).
-  { unfold sched1. exact (J_restrict_only J_bool (mk_single_cpu sched0)). }
-  set (H := deadline_horizon jobs enumJ).
-  destruct (llf_normalize_to_canonical J J_bool candidates_of cand_spec jobs sched1 H
-               HJbool Hvalid1 Hfeas1 HJonly1 Hcpu1)
-    as [sched2 [Hvalid2 [Hfeas2 [HJonly2 [Hcpu2 Hcanon2]]]]].
-  set (sched3 := trunc_sched sched2 H).
-  assert (Hvalid3 : valid_schedule jobs 1 sched3)
-    by (unfold sched3; exact (trunc_sched_valid jobs sched2 H Hvalid2)).
-  assert (Hfeas3 : feasible_schedule_on J jobs 1 sched3).
-  { unfold sched3.
-    apply (trunc_sched_feasible J jobs sched2 H).
-    - intros j HJj. apply Nat.lt_le_incl.
-      unfold H. exact (J_implies_deadline_lt_horizon J enumJ jobs j HJ_in HJj).
-    - exact Hfeas2. }
-  assert (Hcpu3 : single_cpu_only sched3).
-  { unfold sched3. exact (trunc_sched_single_cpu_only sched2 H Hcpu2). }
-  assert (Hcanon3 : matches_choose_llf_before jobs candidates_of sched3 H).
-  { unfold sched3.
-    exact (trunc_sched_llf_canonical J candidates_of cand_spec jobs sched2 H
-             Hcpu2 (trunc_sched_single_cpu_only sched2 H Hcpu2) Hcanon2). }
-  assert (Hidle3 : forall t, H <= t -> sched3 t 0 = None).
-  { intros t Hle. unfold sched3.
-    exact (trunc_sched_after sched2 H t 0 Hle). }
-  assert (Hrel : scheduler_rel (llf_scheduler candidates_of) jobs 1 sched3).
-  { exact (canonical_and_idle_implies_scheduler_rel_llf J enumJ candidates_of cand_spec
-             jobs sched3 HJ_in Hvalid3 Hfeas3 Hcpu3 Hcanon3 Hidle3). }
-  exact (single_cpu_algorithm_schedulable_by_on_intro J llf_generic_spec candidates_of
-           cand_spec jobs sched3 Hrel Hfeas3).
+         HJbool HJ_in _HJ_complete Hfeas_on.
+  change (schedulable_by_on
+            J
+            (single_cpu_algorithm_scheduler_on J llf_generic_spec candidates_of cand_spec)
+            jobs 1).
+  eapply finite_optimality_via_normalization.
+  - exact HJbool.
+  - exact HJ_in.
+  - intros sched0 H Hvalid Hfeas HJonly Hcpu.
+    exact (llf_normalize_to_canonical J J_bool candidates_of cand_spec jobs sched0 H
+             HJbool Hvalid Hfeas HJonly Hcpu).
+  - intros s1 s2 t Hagree.
+    exact (llf_dispatch_agrees_before J candidates_of cand_spec jobs s1 s2 t Hagree).
+  - exact Hfeas_on.
 Qed.
