theories/SchedulingAlgorithmNormalization.v
@@ -1,0 +1,114 @@
+From Stdlib Require Import List Bool Arith Arith.PeanoNat Lia.
+Require Import Base.
+Require Import ScheduleModel.
+Require Import ScheduleLemmas.SchedulePrefix.
+Require Import ScheduleLemmas.ScheduleRestriction.
+Require Import SchedulingAlgorithmInterface.
+Require Import SchedulingAlgorithmSchedulerBridge.
+Require Import SchedulingAlgorithmCanonicalBridge.
+Import ListNotations.
+
+Record CanonicalRepairSpec
+    (alg : GenericSchedulingAlgorithm)
+    (J : JobId -> Prop)
+    (candidates_of : CandidateSource)
+    (jobs : JobId -> Job) : Type := {
+  canonical_at : Schedule -> Time -> Prop;
+  canonical_before : Schedule -> Time -> Prop;
+
+  canonical_before_def :
+    forall sched H,
+      canonical_before sched H <->
+      matches_dispatch_before alg jobs candidates_of sched H;
+
+  canonical_at_def :
+    forall sched t,
+      canonical_at sched t <->
+      matches_dispatch_at_with alg jobs candidates_of sched t;
+
+  canonical_at_dec :
+    forall sched t,
+      {canonical_at sched t} + {~ canonical_at sched t};
+
+  repair_non_canonical :
+    forall (J_bool : JobId -> bool) sched t,
+      (forall x, J_bool x = true <-> J x) ->
+      valid_schedule jobs 1 sched ->
+      feasible_schedule_on J jobs 1 sched ->
+      (forall t' j, sched t' 0 = Some j -> J j) ->
+      single_cpu_only sched ->
+      ~ canonical_at sched t ->
+      exists sched',
+        valid_schedule jobs 1 sched' /\
+        feasible_schedule_on J jobs 1 sched' /\
+        (forall t' j, sched' t' 0 = Some j -> J j) /\
+        single_cpu_only sched' /\
+        agrees_before sched sched' t /\
+        canonical_at sched' t;
+
+  repair_pushes_forward :
+    forall sched sched' t,
+      single_cpu_only sched ->
+      single_cpu_only sched' ->
+      agrees_before sched sched' t ->
+      canonical_at sched' t ->
+      canonical_before sched t ->
+      canonical_before sched' (S t)
+}.
+
+Lemma normalize_to_canonical_generic :
+  forall alg J (J_bool : JobId -> bool)
+         (candidates_of : CandidateSource)
+         (cand_spec : CandidateSourceSpec J candidates_of)
+         jobs sched H,
+    CanonicalRepairSpec alg J candidates_of jobs ->
+    (forall x, J_bool x = true <-> J x) ->
+    valid_schedule jobs 1 sched ->
+    feasible_schedule_on J jobs 1 sched ->
+    (forall t j, sched t 0 = Some j -> J j) ->
+    single_cpu_only sched ->
+    exists sched',
+      valid_schedule jobs 1 sched' /\
+      feasible_schedule_on J jobs 1 sched' /\
+      (forall t j, sched' t 0 = Some j -> J j) /\
+      single_cpu_only sched' /\
+      matches_dispatch_before alg jobs candidates_of sched' H.
+Proof.
+  intros alg J J_bool candidates_of cand_spec jobs sched H Hspec HJbool.
+  destruct Hspec as [canonical_at canonical_before
+                      Hbefore_def Hat_def Hdec Hrepair Hpush].
+  induction H as [| H' IH].
+  - intros Hvalid Hfeas HJonly Hcpu.
+    exists sched.
+    refine (conj Hvalid (conj Hfeas (conj HJonly (conj Hcpu _)))).
+    unfold matches_dispatch_before.
+    intros t Hlt. lia.
+  - intros Hvalid Hfeas HJonly Hcpu.
+    destruct (IH Hvalid Hfeas HJonly Hcpu)
+      as [sched_ih [Hvalid_ih [Hfeas_ih [HJonly_ih [Hcpu_ih Hcanon_ih]]]]].
+    assert (Hbefore_ih : canonical_before sched_ih H').
+    { apply (proj2 (Hbefore_def sched_ih H')).
+      exact Hcanon_ih. }
+    destruct (Hdec sched_ih H') as [Hat | Hnot].
+    + exists sched_ih.
+      refine (conj Hvalid_ih (conj Hfeas_ih (conj HJonly_ih (conj Hcpu_ih _)))).
+      apply (proj1 (Hbefore_def sched_ih (S H'))).
+      eapply Hpush.
+      * exact Hcpu_ih.
+      * exact Hcpu_ih.
+      * apply agrees_before_refl.
+      * exact Hat.
+      * exact Hbefore_ih.
+    + destruct (Hrepair J_bool sched_ih H'
+                  HJbool Hvalid_ih Hfeas_ih HJonly_ih Hcpu_ih Hnot)
+        as [sched_r [Hvalid_r [Hfeas_r [HJonly_r [Hcpu_r [Hagree Hat_r]]]]]].
+      exists sched_r.
+      refine (conj Hvalid_r (conj Hfeas_r (conj HJonly_r (conj Hcpu_r _)))).
+      apply (proj1 (Hbefore_def sched_r (S H'))).
+      eapply Hpush.
+      * exact Hcpu_ih.
+      * exact Hcpu_r.
+      * exact Hagree.
+      * exact Hat_r.
+      * exact Hbefore_ih.
+Qed.
