theories/SchedulingAlgorithmOptimalitySkeleton.v
@@ -1,0 +1,157 @@
+From Stdlib Require Import List Bool Arith Arith.PeanoNat Lia.
+Require Import Base.
+Require Import ScheduleModel.
+Require Import ScheduleLemmas.SchedulePrefix.
+Require Import ScheduleLemmas.ScheduleRestriction.
+Require Import ScheduleLemmas.ScheduleTruncation.
+Require Import SchedulerInterface.
+Require Import SchedulingAlgorithmInterface.
+Require Import SchedulingAlgorithmSchedulerBridge.
+Require Import SchedulingAlgorithmCanonicalBridge.
+Import ListNotations.
+
+Lemma finite_J_restricted_schedule :
+  forall J (J_bool : JobId -> bool) jobs,
+    (forall x, J_bool x = true <-> J x) ->
+    feasible_on J jobs 1 ->
+    exists sched1,
+      valid_schedule jobs 1 sched1 /\
+      feasible_schedule_on J jobs 1 sched1 /\
+      (forall t j, sched1 t 0 = Some j -> J j) /\
+      single_cpu_only sched1.
+Proof.
+  intros J J_bool jobs HJbool [sched0 [Hvalid0 Hfeas0]].
+  exists (J_restrict J_bool (mk_single_cpu sched0)).
+  refine (conj _ (conj _ (conj _ _))).
+  - apply (J_restrict_valid J_bool J jobs (mk_single_cpu sched0) HJbool).
+    exact (mk_single_cpu_valid jobs sched0 Hvalid0).
+  - apply (J_restrict_feasible J_bool J jobs (mk_single_cpu sched0) HJbool).
+    exact (mk_single_cpu_feasible J jobs sched0 Hfeas0).
+  - intros t j Hrun.
+    exact (J_restrict_J_only J_bool J (mk_single_cpu sched0) t j HJbool Hrun).
+  - exact (J_restrict_only J_bool (mk_single_cpu sched0)).
+Qed.
+
+Lemma finite_normalized_schedule :
+  forall alg J (J_bool : JobId -> bool) candidates_of jobs sched1 H,
+    (forall sched0 H0,
+        valid_schedule jobs 1 sched0 ->
+        feasible_schedule_on J jobs 1 sched0 ->
+        (forall t j, sched0 t 0 = Some j -> J j) ->
+        single_cpu_only sched0 ->
+        exists sched',
+          valid_schedule jobs 1 sched' /\
+          feasible_schedule_on J jobs 1 sched' /\
+          (forall t j, sched' t 0 = Some j -> J j) /\
+          single_cpu_only sched' /\
+          matches_dispatch_before alg jobs candidates_of sched' H0) ->
+    valid_schedule jobs 1 sched1 ->
+    feasible_schedule_on J jobs 1 sched1 ->
+    (forall t j, sched1 t 0 = Some j -> J j) ->
+    single_cpu_only sched1 ->
+    exists sched2,
+      valid_schedule jobs 1 sched2 /\
+      feasible_schedule_on J jobs 1 sched2 /\
+      (forall t j, sched2 t 0 = Some j -> J j) /\
+      single_cpu_only sched2 /\
+      matches_dispatch_before alg jobs candidates_of sched2 H.
+Proof.
+  intros alg J J_bool candidates_of jobs sched1 H Hnorm Hvalid1 Hfeas1 HJonly1 Hcpu1.
+  exact (Hnorm sched1 H Hvalid1 Hfeas1 HJonly1 Hcpu1).
+Qed.
+
+Lemma finite_truncated_schedule :
+  forall alg J enumJ candidates_of
+         (cand_spec : CandidateSourceSpec J candidates_of)
+         jobs sched2,
+    (forall s1 s2 t,
+        agrees_before s1 s2 t ->
+        dispatch alg jobs 1 s1 t (candidates_of jobs 1 s1 t) =
+        dispatch alg jobs 1 s2 t (candidates_of jobs 1 s2 t)) ->
+    (forall j, J j -> In j enumJ) ->
+    valid_schedule jobs 1 sched2 ->
+    feasible_schedule_on J jobs 1 sched2 ->
+    single_cpu_only sched2 ->
+    matches_dispatch_before alg jobs candidates_of sched2 (deadline_horizon jobs enumJ) ->
+    exists sched3,
+      valid_schedule jobs 1 sched3 /\
+      feasible_schedule_on J jobs 1 sched3 /\
+      single_cpu_only sched3 /\
+      matches_dispatch_before alg jobs candidates_of sched3 (deadline_horizon jobs enumJ) /\
+      (forall t, deadline_horizon jobs enumJ <= t -> sched3 t 0 = None).
+Proof.
+  intros alg J enumJ candidates_of cand_spec jobs sched2 Hdispatch HJ_in
+         Hvalid2 Hfeas2 Hcpu2 Hcanon2.
+  exists (trunc_sched sched2 (deadline_horizon jobs enumJ)).
+  refine (conj _ (conj _ (conj _ (conj _ _)))).
+  - exact (trunc_sched_valid jobs sched2 (deadline_horizon jobs enumJ) Hvalid2).
+  - apply (trunc_sched_feasible J jobs sched2 (deadline_horizon jobs enumJ) Hfeas2).
+    intros j HJj.
+    exact (J_implies_deadline_le_horizon J enumJ jobs j HJ_in HJj).
+  - exact (trunc_sched_single_cpu_only sched2 (deadline_horizon jobs enumJ) Hcpu2).
+  - eapply trunc_sched_preserves_canonical_before; eauto.
+  - intros t Hle.
+    exact (trunc_sched_after sched2 (deadline_horizon jobs enumJ) t 0 Hle).
+Qed.
+
+Lemma finite_canonical_schedule_yields_scheduler_rel :
+  forall alg J enumJ candidates_of
+         (cand_spec : CandidateSourceSpec J candidates_of)
+         jobs sched3,
+    (forall j, J j -> In j enumJ) ->
+    valid_schedule jobs 1 sched3 ->
+    feasible_schedule_on J jobs 1 sched3 ->
+    single_cpu_only sched3 ->
+    matches_dispatch_before alg jobs candidates_of sched3 (deadline_horizon jobs enumJ) ->
+    (forall t, deadline_horizon jobs enumJ <= t -> sched3 t 0 = None) ->
+    scheduler_rel (single_cpu_algorithm_schedule alg candidates_of) jobs 1 sched3.
+Proof.
+  intros alg J enumJ candidates_of cand_spec jobs sched3
+         HJ_in Hvalid3 Hfeas3 Hcpu3 Hcanon3 Hidle3.
+  eapply canonical_and_idle_implies_scheduler_rel_generic; eauto.
+Qed.
+
+Theorem finite_optimality_via_normalization :
+  forall alg J (J_bool : JobId -> bool) enumJ
+         (candidates_of : CandidateSource)
+         (cand_spec : CandidateSourceSpec J candidates_of)
+         jobs,
+    (forall x, J_bool x = true <-> J x) ->
+    (forall j, J j -> In j enumJ) ->
+    (forall sched0 H,
+        valid_schedule jobs 1 sched0 ->
+        feasible_schedule_on J jobs 1 sched0 ->
+        (forall t j, sched0 t 0 = Some j -> J j) ->
+        single_cpu_only sched0 ->
+        exists sched',
+          valid_schedule jobs 1 sched' /\
+          feasible_schedule_on J jobs 1 sched' /\
+          (forall t j, sched' t 0 = Some j -> J j) /\
+          single_cpu_only sched' /\
+          matches_dispatch_before alg jobs candidates_of sched' H) ->
+    (forall s1 s2 t,
+        agrees_before s1 s2 t ->
+        dispatch alg jobs 1 s1 t (candidates_of jobs 1 s1 t) =
+        dispatch alg jobs 1 s2 t (candidates_of jobs 1 s2 t)) ->
+    feasible_on J jobs 1 ->
+    schedulable_by_on
+      J
+      (single_cpu_algorithm_scheduler_on J alg candidates_of cand_spec)
+      jobs 1.
+Proof.
+  intros alg J J_bool enumJ candidates_of cand_spec jobs
+         HJbool HJ_in Hnorm Hdispatch Hfeas_on.
+  destruct (finite_J_restricted_schedule J J_bool jobs HJbool Hfeas_on)
+    as [sched1 [Hvalid1 [Hfeas1 [HJonly1 Hcpu1]]]].
+  destruct (finite_normalized_schedule alg J J_bool candidates_of jobs sched1
+              (deadline_horizon jobs enumJ) Hnorm Hvalid1 Hfeas1 HJonly1 Hcpu1)
+    as [sched2 [Hvalid2 [Hfeas2 [HJonly2 [Hcpu2 Hcanon2]]]]].
+  destruct (finite_truncated_schedule alg J enumJ candidates_of cand_spec jobs sched2
+              Hdispatch HJ_in Hvalid2 Hfeas2 Hcpu2 Hcanon2)
+    as [sched3 [Hvalid3 [Hfeas3 [Hcpu3 [Hcanon3 Hidle3]]]]].
+  assert (Hrel :
+            scheduler_rel (single_cpu_algorithm_schedule alg candidates_of) jobs 1 sched3).
+  { eapply finite_canonical_schedule_yields_scheduler_rel; eauto. }
+  exact (single_cpu_algorithm_schedulable_by_on_intro
+           J alg candidates_of cand_spec jobs sched3 Hrel Hfeas3).
+Qed.
